$$
\dot{\rho} = -3H(\rho + P)
$$

$$
H^2:=\left(\frac{\dot{a}}{a}\right)^2=\frac{8\pi G}{3c^2}\rho - \frac{kc^2}{a^2}
$$

$$
P=w\rho
$$

$$
a(t) = a_o\left[\frac{2}{3}\left(\frac{8\pi G\rho_0}{3c^2}\right)^{\frac{1}{2}}\left(1+w\right)\left(t-t_0\right)+1\right]^{\frac{2}{3\left(1+w\right)}}
$$

$$
\Delta t = \frac{\frac{2}{3}H_0}{1+w}
$$

$$
\rho + 3P \leq 0
$$

$$
\left(\frac{\dot{a}}{a}\right)^2=\frac{8\pi G}{3c^2}\rho_0\left(\frac{a}{a_0}\right)^{-3(1+w)} - \frac{kc^2}{a^2}
$$

$$
g_{tt}=1\\
g_{rr}=\frac{a^2}{1-kr}\\
$$


\begin{align*}
    g_{tt}&=1\\
    g_{rr}&=\frac{a^2}{1-kr}\\
    g_{\theta\theta}&=a^2r^2\\
    g_{\phi\phi}&=a^2r^2\sin^2\theta
\end{align*}

\begin{align*}
    R_{tt}&=-\frac{a\ddot{a}}{a}\\
    R_{ii}&=-\frac{g_{ii}}{a^2}\left(a\ddot{a}+2\dot{a}^2+2k\right)
\end{align*}

\begin{align*}
    R = -6\left[\frac{\ddot{a}}{a}+\left(\frac{\dot{a}}{a}\right)^2+\frac{k}{a^2}\right]
\end{align*}

\begin{align*}
    T_{tt}&=\rho\\
    T_{ii}&=-Pg_{ii}
\end{align*}

\begin{align*}
    R_{\mu\nu}-\frac{1}{2}g_{\mu\nu}R-\Lambda g_{\mu\nu} = \kappa T_{\mu\nu}
\end{align*}

\begin{align*}
    \left(\frac{\dot{a}}{a}\right)^2&=\frac{\Lambda}{3}-\frac{k}{a^2}\\
    \dot{a}&=\left(\frac{\Lambda}{3}a^2-k\right)^{1/2}
\end{align*}

\begin{align*}
    \left(\frac{\dot{a}}{a}\right)^2=\frac{8\pi G}{3c^2}\rho_0\left(\frac{a_0}{a}\right)^{3(1+w)}+\frac{\Lambda}{3}
\end{align*}